basis/stdoutFFIScript.sml
@@ -14,7 +14,16 @@ val ffi_putChar_length = Q.store_thm("ffi_putChar_length",
   EVAL_TAC \\ every_case_tac \\ rw[] \\ Cases_on`bytes` \\ fs[NULL_EQ]
   \\ Cases_on`t` \\ fs[]);
 
+val ffi_writeStr_def = Define`
+    ffi_writeStr (conf:word8 list) (bytes:word8 list) out =
+      SOME (bytes, out ++ TAKE 65535 (MAP (CHR o w2n) conf))`
+
+val ffi_write_length = Q.store_thm("ffi_writeStr_length",
+  `ffi_write conf bytes out = SOME (bytes',out') ⇒ LENGTH bytes' = LENGTH bytes`,
+  EVAL_TAC \\ every_case_tac \\ rw[] \\ Cases_on`bytes` \\ fs[NULL_EQ]
+  \\ Cases_on`t` \\ fs[]);
+
 val stdout_ffi_part_def = Define`
-  stdout_ffi_part = (Str, destStr, [("putChar",ffi_putChar)])`;
+  stdout_ffi_part = (Str, destStr, [("putChar",ffi_putChar);("writeStr",ffi_writeStr)])`;
 
 val _ = export_theory();
